making some progress on even index sorting

crypto_examples/index.dfy
@@ -1,12 +1,5 @@
 include "omega.dfy"
-include "../std_lib/src/Collections/Sequences/LittleEndianNat.dfy"
-
-module bins refines LittleEndianNat {
-    function method BASE(): nat
-    {
-        2
-    }
-}
+include "bins.dfy"
 
 module rindex {
     import opened Power
@@ -22,8 +15,8 @@ module rindex {
 
     predicate valid_index(idx: index_raw)
     {
+        && 1 <= idx.bound.exp == |idx.bins| // exp is the number of bits, we have at least 1 bit
         && idx.v < idx.bound.full
-        && |idx.bins| == idx.bound.exp // exp is the number of bits
         && idx.v == ToNatRight(idx.bins)
     }
 
@@ -37,7 +30,6 @@ module rindex {
     }
 
     lemma valid_index_correspondence(idx: index_t)
-        requires 1 <= idx.bound.exp 
         ensures idx.v % 2 == First(idx.bins);
         ensures idx.v / 2 == ToNatRight(DropFirst(idx.bins));
     {
@@ -49,10 +41,20 @@ module rindex {
         assert v' == ToNatRight(bins');
     }
 
-    function method reverse_bits(idx: index_t): (new_idx: index_raw)
-        requires 1 <= idx.bound.exp < N == Pow(2, L);
+    function method lsb(idx: index_t): (lsb: uint1)
+        ensures lsb == First(idx.bins);
+    {
+        valid_index_correspondence(idx);
+        idx.v % 2
+    }
+
+    function method bit_rev_index(idx: index_t): (new_idx: index_raw)
+        requires idx.bound.exp < N == Pow(2, L);
         ensures valid_index(new_idx);
-        decreases idx.bound.exp
+        ensures new_idx.bins == Reverse(idx.bins);
+        // ensures forall i: 0 <= i < |idx.bin| ==>
+        //     new_idx.bin[i] == idx.bin[idx.bound.full - i - 1];
+        decreases idx.bound.exp;
     {
         if idx.bound.exp == 1 then idx
         else pow2_basics(idx.bound);
@@ -61,7 +63,7 @@ module rindex {
             var bins' := DropFirst(idx.bins);
             valid_index_correspondence(idx);
             var temp := index_cons(v', bins', bound');
-            var idx' := reverse_bits(temp);
+            var idx' := bit_rev_index(temp);
             valid_index_correspondence(idx');
             assert idx'.v + lsb * bound'.full == ToNatRight(idx'.bins + [lsb]) by {
                 calc == {
@@ -84,6 +86,94 @@ module rindex {
             assert idx'.v + lsb * bound'.full < idx.bound.full by {
                 LemmaSeqNatBound(idx'.bins + [lsb]);
             }
+            assert idx'.bins + [lsb] == Reverse(idx.bins) by {
+                reveal Reverse();
+            }
             index_cons(idx'.v + lsb * bound'.full, idx'.bins + [lsb], idx.bound)
+    }
+
+    predicate ntt_indicies_wf(idxs: seq<index_t>, len: pow2_t)
+    {
+        && len.exp <= L
+        && |idxs| == len.full
+        && (forall i: nat :: i < len.full ==> 
+            idxs[i].bound == pow2(L))
+    }
+
+    predicate ntt_indicies_inv(idxs: seq<index_t>, len: pow2_t)
+    {
+        && ntt_indicies_wf(idxs, len)
+        && (forall i: nat :: i < len.full ==> 
+            ToNatRight(idxs[i].bins[(L - len.exp)..]) == i)
+    }
+
+    lemma ntt_indicies_inv_base_case(idxs: seq<index_t>, len: pow2_t)
+        requires len == pow2(L)
+        requires ntt_indicies_wf(idxs, len)
+        requires forall i: nat :: i < len.full ==> idxs[i].v == i;
+        requires ntt_indicies_inv(idxs, len)
+    {
+        forall i: nat | i < len.full
+            ensures ToNatRight(idxs[i].bins[0..]) == i
+        {
+            calc == {
+                ToNatRight(idxs[i].bins[0..]);
+                ToNatRight(idxs[i].bins);
+                idxs[i].v;
+                i;
+            }
+        }
+    }
+
+    function method even_indexed_indices(idxs: seq<index_t>, len: pow2_t): (idx': seq<index_t>)
+        requires |idxs| == len.full >= 2;
+        ensures |idx'| == len.full / 2;
+    {
+        pow2_basics(len);
+        seq(len.full/2, n requires 0 <= n < len.full/2 => idxs[n * 2])
+    }
+
+    lemma even_indexed_indices_reorder(idxs: seq<index_t>, len: pow2_t, idxs': seq<index_t>)
+        requires len.full >= 2;
+        requires ntt_indicies_inv(idxs, len); 
+        requires even_indexed_indices(idxs, len) == idxs';
+        ensures ntt_indicies_inv(idxs', pow2_half(len));
+    {
+        var len' := pow2_half(len);
+        assert ntt_indicies_wf(idxs', len');
+
+        forall i: nat | i < len'.full
+            ensures ToNatRight(idxs'[i].bins[(L - len'.exp)..]) == i
+        {
+            var bins := idxs[i * 2].bins;
+            assert bins == idxs'[i].bins;
+
+            var offset := L - len.exp;
+            var prev := bins[offset..];
+            var curr := bins[offset+1..];
+
+            calc == {
+                2 * i;
+                ToNatRight(prev);
+                {
+                    assert [bins[offset]] + curr == prev;
+                    assert DropFirst(prev) == curr;
+                    reveal ToNatRight();
+                }
+                ToNatRight(curr) * 2 + bins[offset];
+                {
+                    LemmaSeqLswModEquivalence(prev);
+                    assert ToNatRight(prev) == 2 * i;
+                    assert bins[offset] == 0;
+                }
+                ToNatRight(curr) * 2;
+            }
+
+            calc == {
+                i;
+                ToNatRight(curr);
+                ToNatRight(idxs'[i].bins[(L - len'.exp)..]);
+            }
+        }
     }
 }
