crypto_examples/bins.dfy
@@ -1,0 +1,8 @@
+include "../std_lib/src/Collections/Sequences/LittleEndianNat.dfy"
+
+module bins refines LittleEndianNat {
+    function method BASE(): nat
+    {
+        2
+    }
+}
